ems/ModSemProof.v
@@ -1,0 +1,724 @@
+Require Import Coqlib.
+Require Export sflib.
+Require Export ITreelib.
+Require Import STS Behavior.
+Require Import ModSem.
+Require Import SimGlobal.
+Require Import Skeleton.
+Require Import STS Behavior.
+Require Import Any.
+Require Import Optics.
+
+Set Implicit Arguments.
+
+Module ModSemAdd.
+Import ModSem.
+
+Section ADD.
+  Variable M1 M2 : t.
+
+  Definition emb_l : forall X, Es (state M1) X -> Es (state M1 * state M2) X  :=
+    lmap fstl.
+
+  Definition emb_r : forall X, Es (state M2) X -> Es (state M1 * state M2) X :=
+    lmap sndl.
+
+  Definition add_fnsems : gname -> option (Any.t -> itree _ Any.t) :=
+    fun fn =>
+      match M1.(fnsems) fn, M2.(fnsems) fn with
+      | Some fn_body, None => Some (fun args => translate emb_l (fn_body args))
+      | None, Some fn_body => Some (fun args => translate emb_r (fn_body args))
+      | Some _, Some _ => Some (fun args => triggerUB)
+      | _, _ => None
+      end.
+
+  Definition add : t :=
+  {|
+    state := state M1 * state M2;
+    init_st := (init_st M1, init_st M2);
+    fnsems := add_fnsems;
+  |}.
+
+End ADD.
+
+Section PROOF.
+
+Lemma interp_Es_vis
+T R st p (st0: st)
+(* (e: Es Σ) *)
+(c: callE T) (k: T -> itree (Es st) R)
+:
+interp_Es p (Vis (c|)%sum k) st0 = tau;; (interp_Es p (ITree.bind (p _ c) k) st0) 
+.
+Proof. 
+unfold interp_Es, interp_sE.
+rewrite interp_mrec_bind. grind.
+Admitted. 
+
+
+Context {CONF: EMSConfig}.
+
+Let add_comm_aux
+    ms0 ms1 stl0 str0
+    P
+    (SIM: stl0 = str0)
+  :
+    <<COMM: Beh.of_state (compile (add ms0 ms1) P) stl0
+            <1=
+            Beh.of_state (compile (add ms1 ms0) P) str0>>
+.
+Proof.
+  subst. revert str0. pcofix CIH. i. pfold.
+  punfold PR. induction PR using Beh.of_state_ind; ss.
+  - econs 1; et.
+  - econs 2; et.
+    clear CIH. clear_tac. revert st0 H.
+    pcofix CIH. i. punfold H0. pfold.
+    inv H0.
+    + econs 1; eauto. ii. ss. exploit STEP; et. i; des. right. eapply CIH; et. pclearbot. ss.
+    + econs 2; eauto. des. esplits; eauto. right. eapply CIH; et. pclearbot. ss.
+  - econs 4; et. pclearbot. right. eapply CIH; et.
+  - econs 5; et. rr in STEP. des. rr. esplits; et.
+  - econs 6; et. ii. exploit STEP; et. i; des. clarify.
+Qed.
+
+Theorem add_comm
+        ms0 ms1
+        (P0 P1: Prop) (IMPL: P1 -> P0)
+        (* (WF: wf (add ms1 ms0)) *)
+  :
+    <<COMM: Beh.of_program (compile (add ms0 ms1) (Some P0)) <1= Beh.of_program (compile (add ms1 ms0) (Some P1))>>
+.
+Proof.
+
+  destruct (classic (P1)); cycle 1.
+  { ii. eapply initial_itr_not_wf;et. }
+  replace P0 with P1.
+  2: { eapply prop_ext. split; auto. }
+  
+
+
+  unfold compile. red. apply adequacy_global_itree; et.
+  ginit. apply cpn7_wcompat. apply simg_mon.
+  unfold initial_itr, assume. generalize "main" as fn. i.
+  rewrite ! bind_bind. 
+  guclo simg_indC_spec. eapply simg_indC_takeL; et. i. 
+  guclo simg_indC_spec. eapply simg_indC_takeR; et. exists x.
+  rewrite ! bind_ret_l. gcofix CIH.
+  unfold "<$>". simpl. unfold ITree.map.
+  rewrite ! interp_Es_bind. rewrite ! bind_bind.
+  unfold unwrapU, add_fnsems. 
+  des_ifs.
+
+  - rewrite ! interp_Es_ret. grind. 
+    rewrite interp_Es_triggerUB. unfold triggerUB. grind.
+    gstep. econs; et. i. destruct x0.
+  - rewrite ! interp_Es_ret. grind.
+    generalize (i1 initial_arg). gcofix CIH'. i.
+
+    rewrite (itree_eta_ i).
+    destruct (observe i).
+    +(* Ret *)
+      rewrite (bisimulation_is_eq _ _ (translate_ret (emb_r ms1 ms0) r0)).
+      rewrite (bisimulation_is_eq _ _ (translate_ret (emb_l ms0 ms1) r0)).
+      rewrite ! interp_Es_ret. rewrite ! bind_ret_l.
+      gstep. econs. et.
+    + (* Tau *)
+      rewrite (bisimulation_is_eq _ _ (translate_tau (emb_r ms1 ms0) t0)).
+      rewrite (bisimulation_is_eq _ _ (translate_tau (emb_l ms0 ms1) t0)).
+      rewrite ! interp_Es_tau. rewrite ! bind_tau.
+      gstep. econs; et. econs; et. (* -> Can go back to gpaco without flag change? *) 
+      (* econs; et. gfinal. left. apply CIH'. *)
+      admit.
+    + (* Vis *)
+      rewrite (bisimulation_is_eq _ _ (translate_vis (emb_r ms1 ms0) _ e k)).
+      rewrite (bisimulation_is_eq _ _ (translate_vis (emb_l ms0 ms1) _ e k)).
+      destruct e.
+      * unfold emb_r at 1. unfold emb_l at 1. unfold lmap.
+        rewrite ! interp_Es_vis. destruct c. grind.
+        guclo simg_indC_spec. apply simg_indC_tauL; et.
+        guclo simg_indC_spec. apply simg_indC_tauR; et.
+        unfold "<$>" in CIH. simpl in CIH. unfold ITree.map in CIH.
+
+
+
+
+  destruct (fnsems ms0 fn); cycle 1. 
+  { 
+    destruct (fnsems ms1 fn); cycle 1.
+    - rewrite ! interp_Es_triggerUB.
+      unfold triggerUB. grind.
+      guclo simg_indC_spec. eapply simg_indC_takeL; et. i.
+      destruct x0.
+    - rewrite ! interp_Es_ret. rewrite ! bind_ret_l.
+      rewrite ! interp_Es_bind. grind.
+      generalize (i initial_arg).
+      gcofix CIH'. i.
+      
+      rewrite (itree_eta_ i0).
+      destruct (observe i0).
+      3: {
+        rewrite (bisimulation_is_eq _ _ (translate_vis (emb_l ms1 ms0) _ e k)).
+        rewrite (bisimulation_is_eq _ _ (translate_vis (emb_r ms0 ms1) _ e k)).
+        destruct e.
+        {
+          (* unfold "<$>" in CIH. simpl in CIH. unfold ITree.map in CIH. *)
+          unfold emb_l, emb_r at 1. unfold lmap at 1 3. 
+          rewrite ! interp_Es_vis. destruct c. grind.
+          (* gstep. econs; et. econs; et. *)
+          guclo simg_indC_spec. apply simg_indC_tauL; et.
+          guclo simg_indC_spec. apply simg_indC_tauR; et.
+          (* gstep. econs; et. gfinal. left. *)
+          
+          rewrite ! interp_Es_bind. grind.
+          rewrite ! interp_Es_unwrapU. grind.
+          unfold unwrapU. des_ifs.
+          + rewrite ! bind_ret_l. rewrite ! interp_Es_bind. grind.
+            
+             
+
+        }
+       } 
+
+  }
+
+
+
+
+  ii. ss. r in PR. r. eapply add_comm_aux. et.
+  rp; et. clear PR. ss. cbn. unfold initial_itr. f_equal.
+  
+  extensionality u. destruct u.
+  apply bisimulation_is_eq. generalize "main" as fn.
+  ginit. gcofix CIH.
+  simpl. unfold ITree.map. repeat (rewrite interp_Es_bind; rewrite bind_bind).  
+  unfold unwrapU. unfold add_fnsems. i.
+  destruct (fnsems ms0 fn); cycle 1.
+  {
+    destruct (fnsems ms1 fn); cycle 1.
+    - rewrite ! interp_Es_bind. rewrite ! interp_Es_triggerUB.
+      gstep. unfold triggerUB. grind. 
+      rewrite ! bind_trigger; s.
+      econs. i. destruct v.  
+    - rewrite ! interp_Es_bind. rewrite ! interp_Es_ret. rewrite ! bind_ret_l.
+      rewrite ! interp_Es_bind. grind.
+      generalize (i initial_arg).
+      gcofix CIH'. i.
+      rewrite (itree_eta_ i0). 
+      destruct (observe i0).
+      + rewrite (bisimulation_is_eq _ _ (translate_ret (emb_l ms1 ms0) r0)).
+        rewrite (bisimulation_is_eq _ _ (translate_ret (emb_r ms0 ms1) r0)).
+        rewrite ! interp_Es_ret. rewrite ! bind_ret_l.
+        rewrite ! interp_Es_ret. rewrite ! bind_ret_l.
+        gstep. econs. et.
+
+      + 
+        rewrite (bisimulation_is_eq _ _ (translate_tau (emb_l ms1 ms0) t0)).
+        rewrite (bisimulation_is_eq _ _ (translate_tau (emb_r ms0 ms1) t0)).
+        rewrite ! interp_Es_tau. rewrite ! bind_tau.
+        gstep. econs. gfinal. left. apply CIH'.
+      + rewrite (bisimulation_is_eq _ _ (translate_vis (emb_l ms1 ms0) _ e k)).
+        rewrite (bisimulation_is_eq _ _ (translate_vis (emb_r ms0 ms1) _ e k)).
+        destruct e.
+        * unfold emb_l, emb_r, lmap. clear CIH'.
+          rewrite ! interp_Es_vis. destruct c.
+          gstep. grind. econs. gupaco.
+          apply eqit_clo_bind; et. Print eqit_bind_clo.
+          econs.
+          { admit. }
+          { admit. }
+        * admit.
+
+       
+          (* right. 
+          apply CIH.
+
+          eassert (Y := (interp_Es_callE _ _ c)).
+          unfold trigger in Y.
+          rewrite interp_Es_bind in Y.
+          unfold subevent in Y. unfold resum, ReSum_inl, ">>>" in Y. 
+          unfold emb_l, lmap. unfold Cat_IFun, inl_, Inl_sum1, resum, ReSum_id, id_, Id_IFun in Y.
+          rewrite Y.
+          Print Subevent.vis. Check subevent.
+          rewrite Y.
+        rewrite (interp_Es_callE _ _ c) (emb_l ms1 ms0 (c|)%sum)). *)
+
+    }
+    {
+      admit.
+    }
+Admitted.
+
+  (* revert ms0 ms1. pcofix CIH. i.
+  pfold.
+
+  simpl. unfold ITree.map. repeat (rewrite interp_Es_bind; rewrite bind_bind).
+  unfold unwrapU. unfold add_fnsems.
+Qed. *)
+
+Lemma add_assoc' ms0 ms1 ms2:
+  add ms0 (add ms1 ms2) = add (add ms0 ms1) ms2.
+Proof. Admitted.
+  (* induction ms2; ss. unfold add. f_equal; ss.
+  { eapply app_assoc. }
+  { eapply app_assoc. }
+Qed. *)
+
+Lemma add_assoc_eq ms0 ms1 ms2
+  :
+    add ms0 (add ms1 ms2) = add (add ms0 ms1) ms2.
+Proof. Admitted.
+  (* unfold add. ss. f_equal.
+  { apply List.app_assoc. }
+  { apply List.app_assoc. }
+Qed. *)
+
+Theorem add_assoc
+        ms0 ms1 ms2 P
+  :
+    <<COMM: Beh.of_program (compile (add ms0 (add ms1 ms2)) P) <1=
+            Beh.of_program (compile (add (add ms0 ms1) ms2) P)>>
+.
+Proof. 
+  rewrite add_assoc_eq. ss.
+Qed.
+
+Theorem add_assoc_rev
+        ms0 ms1 ms2 P
+  :
+    <<COMM: Beh.of_program (compile (add ms0 (add ms1 ms2)) P) <1=
+            Beh.of_program (compile (add (add ms0 ms1) ms2) P)>>
+.
+Proof.
+  rewrite add_assoc_eq. ss.
+Qed.
+
+End PROOF.
+End ModSemAdd.
+
+Module ModAdd.
+Import Mod.
+Section BEH.
+
+Context `{Sk.ld}.
+Context {CONF: EMSConfig}.
+
+(* Definition compile (md: t): semantics :=
+  ModSemL.compile_itree (ModSemL.initial_itr md.(enclose) (Some (wf md))). *)
+
+
+Definition compile (md: t): semantics :=
+  ModSem.compile_itree (ModSem.initial_itr md.(enclose) (Some (wf md))).
+
+
+(*** wf about modsem is enforced in the semantics ***)
+
+Definition add (md0 md1: t): t := {|
+  get_modsem := fun sk =>
+                  ModSem.add (md0.(get_modsem) sk) (md1.(get_modsem) sk);
+  sk := Sk.add md0.(sk) md1.(sk);
+|}
+.
+
+
+(* Definition add (md0 md1: t): t := {|
+  get_modsem := fun sk =>
+                  ModSemL.add (md0.(get_modsem) sk) (md1.(get_modsem) sk);
+  sk := Sk.add md0.(sk) md1.(sk);
+|}
+. *)
+
+Theorem add_comm
+        md0 md1
+  :
+    <<COMM: Beh.of_program (compile (add md0 md1)) <1= Beh.of_program (compile (add md1 md0))>>
+.
+Proof. Admitted.
+  (* ii. unfold compile in *.
+  destruct (classic (Sk.wf (sk (add md1 md0)))).
+  (* 2: { eapply ModSemL.initial_itr_not_wf. ss. } *)
+  ss. des. assert (SK: Sk.wf (Sk.add (sk md0) (sk md1))).
+  { apply Sk.wf_comm. auto. }
+  rewrite Sk.add_comm; et.
+  eapply ModSem.add_comm. [| |et].
+  { i. split; auto. unfold enclose. ss. rewrite Sk.add_comm; et.
+    inv H2. inv H3. econs; ss.
+    { rewrite List.map_app in *. eapply nodup_comm; et. }
+    { rewrite List.map_app in *. eapply nodup_comm; et. }
+  }
+  { rewrite Sk.add_comm; et. }
+Qed. *)
+
+
+
+Lemma add_assoc' ms0 ms1 ms2:
+  add ms0 (add ms1 ms2) = add (add ms0 ms1) ms2.
+Proof.
+  unfold add. f_equal.
+  { extensionality skenv_link. ss. apply ModSem.add_assoc'. }
+  { ss. rewrite Sk.add_assoc. auto. }
+Qed.
+
+Theorem add_assoc
+        md0 md1 md2
+  :
+    <<COMM: Beh.of_program (compile (add md0 (add md1 md2))) =
+            Beh.of_program (compile (add (add md0 md1) md2))>>
+.
+Proof.
+  rewrite add_assoc'. ss.
+Qed.
+
+Theorem add_assoc_rev
+        md0 md1 md2
+  :
+    <<COMM: Beh.of_program (compile (add (add md0 md1) md2)) =
+            Beh.of_program (compile (add md0 (add md1 md2)))>>
+.
+Proof.
+  rewrite add_assoc'. ss.
+Qed.
+
+Lemma add_empty_r 
+      md
+  : 
+    << EMPTY: Beh.of_program (compile (add md empty)) =
+              Beh.of_program (compile md)>>
+.
+Proof. Admitted.
+
+Lemma add_empty_l 
+      md
+  : 
+    << EMPTY: Beh.of_program (compile (add empty md)) =
+              Beh.of_program (compile md)>>
+.
+Proof. Admitted.
+
+
+(* Lemma add_empty_r md: add md empty = md.
+Proof.
+  destruct md; ss.
+  unfold add, ModSem.add. f_equal; ss.
+  - extensionality skenv. destruct (get_modsem0 skenv); ss.
+    repeat rewrite app_nil_r. auto.
+  - eapply Sk.add_unit_r.
+Qed.
+
+Lemma add_empty_l md: add empty md = md.
+Proof.
+  destruct md; ss.
+  unfold add, ModSemL.add. f_equal; ss.
+  { extensionality skenv. destruct (get_modsem0 skenv); ss. }
+  { apply Sk.add_unit_l. }
+Qed. *)
+
+
+Definition add_list (xs: list t): t :=
+  fold_right add empty xs
+.
+
+(* Lemma add_list_single: forall (x: t), add_list [x] = x.
+Proof. ii; cbn. rewrite add_empty_r. refl. Qed. *)
+
+Definition add_list_cons
+          x xs
+        :
+          (add_list (x::xs) = (add x (add_list xs)))
+.
+Proof. ss. Qed.
+(* 
+Definition add_list_snoc
+          x xs
+        :
+          add_list (snoc xs x) = add (add_list xs) x
+.
+Proof. ginduction xs; ii; ss. Admitted. *)
+
+Definition add_list_snoc
+          x xs
+        :
+          << SNOC: Beh.of_program (compile (add_list (snoc xs x))) = 
+                   Beh.of_program (compile (add (add_list xs) x)) >>
+.
+Proof. Admitted.
+  (* ginduction xs; ii; ss.
+  { cbn. rewrite add_empty_l, add_empty_r. et. }
+  { cbn. rewrite <- add_assoc'.  r in IHxs. r. f_equal.}  *)
+
+End BEH.
+End ModAdd.
+
+Section REFINE.
+  Context `{Sk.ld}.
+
+   Definition refines {CONF: EMSConfig} (md_tgt md_src: Mod.t): Prop :=
+     (* forall (ctx: list Mod.t), Beh.of_program (ModL.compile (add_list (md_tgt :: ctx))) <1= *)
+     (*                           Beh.of_program (ModL.compile (add_list (md_src :: ctx))) *)
+     forall (ctx: list Mod.t), Beh.of_program (ModAdd.compile (ModAdd.add (ModAdd.add_list ctx) md_tgt)) <1=
+                               Beh.of_program (ModAdd.compile (ModAdd.add (ModAdd.add_list ctx) md_src))
+   .
+
+   Definition refines_strong (md_tgt md_src: Mod.t): Prop :=
+     forall {CONF: EMSConfig}, refines md_tgt md_src.
+
+
+   Section CONF.
+   Context {CONF: EMSConfig}.
+
+   Definition refines2 (md_tgt md_src: list Mod.t): Prop :=
+     forall (ctx: list Mod.t), Beh.of_program (ModAdd.compile (ModAdd.add (ModAdd.add_list ctx) (ModAdd.add_list md_tgt))) <1=
+                               Beh.of_program (ModAdd.compile (ModAdd.add (ModAdd.add_list ctx) (ModAdd.add_list md_src)))
+   .
+
+   
+   (* Global Program Instance refines2_PreOrder: PreOrder refines2.
+   Next Obligation.
+     ii. ss.
+   Qed.
+   Next Obligation.
+     ii. eapply H0 in PR. eapply H1 in PR. eapply PR.
+   Qed. *)
+
+   (*** vertical composition ***)
+   Global Program Instance refines_PreOrder: PreOrder refines.
+
+   Next Obligation. ii. ss. Qed.
+   Next Obligation. ii. eapply H1. eapply H0. ss. Qed.
+
+
+   Global Program Instance refines_strong_PreOrder: PreOrder refines_strong.
+   Next Obligation. ii. ss. Qed.
+   Next Obligation. ii. eapply H1. eapply H0. ss. Qed.
+
+
+
+   (*** horizontal composition ***)
+   Theorem refines_add
+         (md0_src md0_tgt md1_src md1_tgt: Mod.t)
+         (SIM0: refines md0_tgt md0_src)
+         (SIM1: refines md1_tgt md1_src)
+     :
+       <<SIM: refines (ModAdd.add md0_tgt md1_tgt) (ModAdd.add md0_src md1_src)>>
+   .
+   Proof. Admitted.
+(*    
+     ii. r in SIM0. r in SIM1.
+     (***
+ctx (a0 b0)
+(ctx a0) b0
+(ctx a0) b1
+      ***)
+     rewrite ModAdd.add_assoc in PR.
+     specialize (SIM1 (snoc ctx md0_tgt)). spc SIM1. rewrite ModAdd.add_list_snoc in SIM1.  eapply SIM1 in PR.
+     (***
+ctx (a0 b1)
+(a0 b1) ctx
+a0 (b1 ctx)
+(b1 ctx) a0
+      ***)
+     rewrite <- ModAdd.add_assoc' in PR.
+     eapply ModAdd.add_comm in PR.
+     rewrite <- ModAdd.add_assoc' in PR.
+     eapply ModAdd.add_comm in PR.
+     (***
+(b1 ctx) a1
+a1 (b1 ctx)
+(a1 b1) ctx
+ctx (a1 b1)
+      ***)
+     specialize (SIM0 (cons md1_src ctx)). spc SIM0. rewrite ModAdd.add_list_cons in SIM0. eapply SIM0 in PR.
+     eapply ModAdd.add_comm in PR.
+     rewrite ModAdd.add_assoc' in PR.
+     eapply ModAdd.add_comm in PR.
+     ss.
+   Qed. *)
+
+   Theorem refines_proper_r
+         (mds0_src mds0_tgt: list Mod.t) (ctx: list Mod.t)
+         (SIM0: refines (ModAdd.add_list mds0_tgt) (ModAdd.add_list mds0_src))
+     :
+       <<SIM: refines (ModAdd.add (ModAdd.add_list mds0_tgt) (ModAdd.add_list ctx)) (ModAdd.add (ModAdd.add_list mds0_src) (ModAdd.add_list ctx))>>
+   .
+   Proof. Admitted.
+(*    
+     ii. r in SIM0. rename ctx into xs. rename ctx0 into ys.
+     (***
+ys + (tgt + xs)
+(tgt + xs) + ys
+tgt + (xs + ys)
+(xs + ys) + tgt
+      ***)
+     eapply ModAdd.add_comm in PR.
+     rewrite <- ModAdd.add_assoc' in PR.
+     eapply ModAdd.add_comm in PR.
+     (***
+(xs + ys) + src
+src + (xs + ys)
+(src + xs) + ys
+ys + (src + xs)
+      ***)
+     specialize (SIM0 (xs ++ ys)). spc SIM0. rewrite ModAdd.add_list_app in SIM0. eapply SIM0 in PR.
+     eapply ModAdd.add_comm in PR.
+     rewrite ModAdd.add_assoc' in PR.
+     eapply ModAdd.add_comm in PR.
+     ss.
+   Qed. *)
+
+   Theorem refines_proper_l
+         (mds0_src mds0_tgt: list Mod.t) (ctx: list Mod.t)
+         (SIM0: refines (ModAdd.add_list mds0_tgt) (ModAdd.add_list mds0_src))
+     :
+       <<SIM: refines (ModAdd.add (ModAdd.add_list ctx) (ModAdd.add_list mds0_tgt)) (ModAdd.add (ModAdd.add_list ctx) (ModAdd.add_list mds0_src))>>
+   .
+   Proof. Admitted.
+     (* ii. r in SIM0. rename ctx into xs. rename ctx0 into ys.
+     (***
+ys + (xs + tgt)
+(ys + xs) + tgt
+(ys + xs) + src
+ys + (xs + src)
+      ***)
+     rewrite ModAdd.add_assoc' in PR.
+     specialize (SIM0 (ys ++ xs)). spc SIM0. rewrite ModAdd.add_list_app in SIM0. eapply SIM0 in PR.
+     rewrite <- ModAdd.add_assoc' in PR.
+     ss.
+   Qed.  *)
+
+   Definition refines_closed (md_tgt md_src: Mod.t): Prop :=
+     Beh.of_program (ModAdd.compile md_tgt) <1= Beh.of_program (ModAdd.compile md_src)
+   .
+
+   Global Program Instance refines_closed_PreOrder: PreOrder refines_closed.
+   Next Obligation. ii; ss. Qed.
+   Next Obligation. ii; ss. eapply H1. eapply H0. eauto. Qed.
+
+   Lemma refines_close: refines <2= refines_closed.
+   Proof. ii. specialize (PR nil). ss. unfold ModAdd.add_list in *. ss. rewrite ! ModAdd.add_empty_l in PR. eauto. Qed.
+
+   (*** horizontal composition ***)
+   Theorem refines2_add
+         (s0 s1 t0 t1: list Mod.t)
+         (SIM0: refines2 t0 s0)
+         (SIM1: refines2 t1 s1)
+     :
+       <<SIM: refines2 (t0 ++ t1) (s0 ++ s1)>>
+   .
+   Proof. Admitted.
+(*    
+     ii. r in SIM0. r in SIM1.
+     (***
+ctx (a0 b0)
+(ctx a0) b0
+(ctx a0) b1
+      ***)
+     rewrite ModAdd.add_list_app in PR.
+     rewrite ModAdd.add_assoc in PR.
+     specialize (SIM1 (ctx ++ t0)). spc SIM1. rewrite ModAdd.add_list_app in SIM1. eapply SIM1 in PR.
+     (***
+ctx (a0 b1)
+(a0 b1) ctx
+a0 (b1 ctx)
+(b1 ctx) a0
+      ***)
+     rewrite <- ModAdd.add_assoc' in PR.
+     eapply ModAdd.add_comm in PR.
+     rewrite <- ModAdd.add_assoc' in PR.
+     eapply ModAdd.add_comm in PR.
+     (***
+(b1 ctx) a1
+a1 (b1 ctx)
+(a1 b1) ctx
+ctx (a1 b1)
+      ***)
+     specialize (SIM0 (s1 ++ ctx)). spc SIM0. rewrite ModAdd.add_list_app in SIM0. eapply SIM0 in PR.
+     eapply ModAdd.add_comm in PR.
+     rewrite ModAdd.add_assoc' in PR.
+     eapply ModAdd.add_comm in PR.
+     rewrite ! ModAdd.add_list_app in *.
+     assumption.
+   Qed.  *)
+
+
+   Corollary refines2_pairwise
+             (mds0_src mds0_tgt: list Mod.t)
+             (FORALL: List.Forall2 (fun md_src md_tgt => refines2 [md_src] [md_tgt]) mds0_src mds0_tgt)
+     :
+       refines2 mds0_src mds0_tgt.
+   Proof.
+     induction FORALL; ss.
+     hexploit refines2_add.
+     { eapply H0. }
+     { eapply IHFORALL. }
+     i. ss.
+   Qed.
+
+   Lemma refines2_eq (mds0 mds1: list Mod.t)
+     :
+       refines2 mds0 mds1 <-> refines (ModAdd.add_list mds0) (ModAdd.add_list mds1).
+   Proof.
+     split.
+     { ii. eapply H0. auto. }
+     { ii. eapply H0. auto. }
+   Qed.
+
+   Lemma refines2_app mhd0 mhd1 mtl0 mtl1
+         (HD: refines2 mhd0 mhd1)
+         (TL: refines2 mtl0 mtl1)
+     :
+       refines2 (mhd0++mtl0) (mhd1++mtl1).
+   Proof. Admitted.
+(*    
+     eapply refines2_eq. rewrite ! ModAdd.add_list_app. etrans.
+     { eapply refines_proper_l. eapply refines2_eq. et. }
+     { eapply refines_proper_r. eapply refines2_eq. et. }
+   Qed. *)
+
+   Lemma refines2_cons mhd0 mhd1 mtl0 mtl1
+         (HD: refines2 [mhd0] [mhd1])
+         (TL: refines2 mtl0 mtl1)
+     :
+       refines2 (mhd0::mtl0) (mhd1::mtl1).
+   Proof.
+     eapply (refines2_app HD TL).
+   Qed.
+
+   End CONF.
+
+
+
+   (*** horizontal composition ***)
+   Theorem refines_strong_add
+         (md0_src md0_tgt md1_src md1_tgt: Mod.t)
+         (SIM0: refines_strong md0_tgt md0_src)
+         (SIM1: refines_strong md1_tgt md1_src)
+     :
+       <<SIM: refines_strong (ModAdd.add md0_tgt md1_tgt) (ModAdd.add md0_src md1_src)>>
+   .
+   Proof.
+     intros CONF. eapply (@refines_add CONF); et.
+   Qed.
+
+   Theorem refines_strong_proper_r
+         (mds0_src mds0_tgt: list Mod.t) (ctx: list Mod.t)
+         (SIM0: refines_strong (ModAdd.add_list mds0_tgt) (ModAdd.add_list mds0_src))
+     :
+       <<SIM: refines_strong (ModAdd.add (ModAdd.add_list mds0_tgt) (ModAdd.add_list ctx)) (ModAdd.add (ModAdd.add_list mds0_src) (ModAdd.add_list ctx))>>
+   .
+   Proof.
+     intros CONF. eapply (@refines_proper_r CONF); et.
+   Qed.
+
+   Theorem refines_strong_proper_l
+         (mds0_src mds0_tgt: list Mod.t) (ctx: list Mod.t)
+         (SIM0: refines_strong (ModAdd.add_list mds0_tgt) (ModAdd.add_list mds0_src))
+     :
+       <<SIM: refines_strong (ModAdd.add (ModAdd.add_list ctx) (ModAdd.add_list mds0_tgt)) (ModAdd.add (ModAdd.add_list ctx) (ModAdd.add_list mds0_src))>>
+   .
+   Proof.
+     intros CONF. eapply (@refines_proper_l CONF); et.
+   Qed.
+
+   Lemma refines_strong_refines {CONF: EMSConfig}: refines_strong <2= refines.
+   Proof. ii. eapply PR; et. Qed.
+End REFINE.
